CoqOfRust/alloc/collections.v
@@ -1,0 +1,306 @@
+Require Import CoqOfRust.Monad.
+Require Import CoqOfRust.lib.lib.
+Require CoqOfRust.core.alloc.
+Require CoqOfRust.core.clone.
+
+Module btree. Module map.
+  (* ********STRUCTS******** *)
+  (* 
+  [x] Cursor
+  [x] CursorMut
+  [?] DrainFilter
+  [x] OccupiedError
+  [x] BTreeMap
+  [x] IntoIter
+  [x] IntoKeys
+  [x] IntoValues
+  [x] Iter
+  [x] IterMut
+  [x] Keys
+  [x] OccupiedEntry
+  [x] Range	
+  [x] RangeMut
+  [x] VacantEntry
+  [x] Values
+  [x] ValuesMut
+  *)
+
+  (* 
+  pub struct Cursor<'a, K, V>
+  where
+      K: 'a,
+      V: 'a,
+  { /* private fields */ } 
+  *)
+  Module Cursor.
+    Parameter t : Set -> Set -> Set.
+  End Cursor.
+  Definition Cursor := Cursor.t.
+
+  (* 
+  pub struct CursorMut<'a, K, V, A = Global>
+  where
+      K: 'a,
+      V: 'a,
+  { /* private fields */ }
+  *)
+  Module CursorMut.
+    Parameter t : Set -> Set -> Set -> Set.
+  End CursorMut.
+  Definition CursorMut (K V : Set) (A : option Set) := 
+    CursorMut.t K V (defaultType A alloc.Global).
+
+  (* 
+  pub struct DrainFilter<'a, K, V, F, A = Global>
+  where
+      A: Allocator + Clone,
+      F: 'a + FnMut(&K, &mut V) -> bool,
+  { /* private fields */ }
+  *)
+  Module DrainFilter.
+    Parameter t : forall (K V A : Set) 
+      `{alloc.Allocator.Trait A}
+      `{core.clone.Clone.Trait A},
+      Set.
+  End DrainFilter.
+  Definition DrainFilter (K V : Set) (A : option Set)
+    `{alloc.Allocator.Trait (defaultType A alloc.Global)}
+    `{core.clone.Clone.Trait (defaultType A alloc.Global)}
+    : Set :=
+    DrainFilter.t K V (defaultType A alloc.Global).
+
+  (* 
+  pub struct OccupiedEntry<'a, K, V, A = Global>
+  where
+      A: Allocator + Clone,
+  { /* private fields */ }
+  *)
+  Module OccupiedEntry.
+    Parameter t : forall (K V A : Set) 
+      `{alloc.Allocator.Trait A}
+      `{core.clone.Clone.Trait A},
+      Set.
+  End OccupiedEntry.
+  Definition OccupiedEntry (K V : Set) (A : option Set)
+    `{alloc.Allocator.Trait (defaultType A alloc.Global)}
+    `{core.clone.Clone.Trait (defaultType A alloc.Global)}
+    : Set :=
+    OccupiedEntry.t K V (defaultType A alloc.Global).
+
+  (* 
+  pub struct OccupiedError<'a, K, V, A = Global>
+  where
+      K: 'a,
+      V: 'a,
+      A: Allocator + Clone,
+  {
+      pub entry: OccupiedEntry<'a, K, V, A>,
+      pub value: V,
+  }
+  *)
+  Module OccupiedError.
+    Record t (K V A : Set) 
+      `{alloc.Allocator.Trait A}
+      `{core.clone.Clone.Trait A}
+    : Set := { 
+      entry : OccupiedEntry K V (Some A);
+      value : V;
+    }.
+  End OccupiedError.
+  Definition OccupiedError (K V : Set) (A : option Set)
+    `{alloc.Allocator.Trait (defaultType A alloc.Global)}
+    `{core.clone.Clone.Trait (defaultType A alloc.Global)}
+    : Set :=
+    OccupiedError.t K V (defaultType A alloc.Global).
+  
+  (* 
+  pub struct BTreeMap<K, V, A = Global>
+  where
+      A: Allocator + Clone,
+  { /* private fields */ }
+  *)
+  Module BTreeMap.
+    Parameter t : forall (K V A : Set) 
+      `{alloc.Allocator.Trait A}
+      `{core.clone.Clone.Trait A},
+      Set.
+
+    Module Default.
+      Definition A : Set := alloc.Global.
+    End Default.
+  End BTreeMap.
+  Definition BTreeMap (K V A : Set)
+    `{alloc.Allocator.Trait A} `{core.clone.Clone.Trait A}
+    : Set :=
+    BTreeMap.t K V A.
+
+  (* 
+  pub struct IntoIter<K, V, A = Global>
+  where
+      A: Allocator + Clone,
+  { /* private fields */ }
+  *)
+  Module IntoIter.
+    Parameter t : forall (K V A : Set) 
+      `{alloc.Allocator.Trait A}
+      `{core.clone.Clone.Trait A},
+      Set.
+  End IntoIter.
+  Definition IntoIter (K V : Set) (A : option Set)
+    `{alloc.Allocator.Trait (defaultType A alloc.Global)}
+    `{core.clone.Clone.Trait (defaultType A alloc.Global)}
+    : Set :=
+    IntoIter.t K V (defaultType A alloc.Global).
+
+  (* 
+  pub struct IntoKeys<K, V, A = Global>
+  where
+      A: Allocator + Clone,
+  { /* private fields */ }
+  *)
+  Module IntoKeys.
+    Parameter t : forall (K V A : Set) 
+      `{alloc.Allocator.Trait A}
+      `{core.clone.Clone.Trait A},
+      Set.
+  End IntoKeys.
+  Definition IntoKeys (K V : Set) (A : option Set)
+    `{alloc.Allocator.Trait (defaultType A alloc.Global)}
+    `{core.clone.Clone.Trait (defaultType A alloc.Global)}
+    : Set :=
+    IntoKeys.t K V (defaultType A alloc.Global).
+
+  (* 
+  pub struct IntoValues<K, V, A = Global>
+  where
+      A: Allocator + Clone,
+  { /* private fields */ }
+  *)
+  Module IntoValues.
+    Parameter t : forall (K V A : Set) 
+      `{alloc.Allocator.Trait A}
+      `{core.clone.Clone.Trait A},
+      Set.
+  End IntoValues.
+  Definition IntoValues (K V : Set) (A : option Set)
+    `{alloc.Allocator.Trait (defaultType A alloc.Global)}
+    `{core.clone.Clone.Trait (defaultType A alloc.Global)}
+    : Set :=
+    IntoValues.t K V (defaultType A alloc.Global).
+
+  (* 
+  pub struct Iter<'a, K, V>
+  where
+      K: 'a,
+      V: 'a,
+  { /* private fields */ }
+  *)
+  Module Iter.
+    Parameter t : Set -> Set -> Set.
+  End Iter.
+  Definition Iter := Iter.t.
+  
+  (* 
+  pub struct IterMut<'a, K, V>
+  where
+      K: 'a,
+      V: 'a,
+  { /* private fields */ }
+  *)
+  Module IterMut.
+    Parameter t : Set -> Set -> Set.
+  End IterMut.
+  Definition IterMut := IterMut.t.
+  
+  (* pub struct Keys<'a, K, V> { /* private fields */ } *)
+  Module Keys.
+    Parameter t : Set -> Set -> Set.
+  End Keys.
+  Definition Keys := Keys.t.
+
+  (* 
+  pub struct Range<'a, K, V>
+  where
+      K: 'a,
+      V: 'a,
+  { /* private fields */ }
+  *)
+  Module Range.
+    Parameter t : Set -> Set -> Set.
+  End Range.
+  Definition Range := Range.t.
+
+  (* 
+  pub struct RangeMut<'a, K, V>
+  where
+      K: 'a,
+      V: 'a,
+  { /* private fields */ }
+  *)
+  Module RangeMut.
+    Parameter t : Set -> Set -> Set.
+  End RangeMut.
+  Definition RangeMut := RangeMut.t.
+  
+  (* 
+  pub struct VacantEntry<'a, K, V, A = Global>
+  where
+      A: Allocator + Clone,
+  { /* private fields */ }
+  *)
+  Module VacantEntry.
+    Parameter t : forall (K V A : Set) 
+      `{alloc.Allocator.Trait A}
+      `{core.clone.Clone.Trait A},
+      Set.
+  End VacantEntry.
+  Definition VacantEntry (K V : Set) (A : option Set)
+    `{alloc.Allocator.Trait (defaultType A alloc.Global)}
+    `{core.clone.Clone.Trait (defaultType A alloc.Global)}
+    : Set :=
+    VacantEntry.t K V (defaultType A alloc.Global).
+  
+  (* pub struct Values<'a, K, V> { /* private fields */ } *)
+  Module Values.
+    Parameter t : Set -> Set -> Set.
+  End Values.
+  Definition Values := Values.t.
+  
+  (* pub struct ValuesMut<'a, K, V> { /* private fields */ } *)
+  Module ValuesMut.
+    Parameter t : Set -> Set -> Set.
+  End ValuesMut.
+  Definition ValuesMut := ValuesMut.t.
+  
+  (* ********ENUMS******** *)
+  (* 
+  [?] Entry
+  *)
+
+  (* BUGGED: same as above *)
+  (* 
+  pub enum Entry<'a, K, V, A = Global>
+  where
+      K: 'a,
+      V: 'a,
+      A: Allocator + Clone,
+  {
+      Vacant(VacantEntry<'a, K, V, A>),
+      Occupied(OccupiedEntry<'a, K, V, A>),
+  }
+  *)
+  Module Entry.
+    Inductive t (K V A : Set) 
+      `{alloc.Allocator.Trait A}
+      `{core.clone.Clone.Trait A}
+    : Set := 
+    | Vacant
+    | Occupied
+    .
+  End Entry.
+  Definition Entry (K V : Set) (A : option Set)
+    `{alloc.Allocator.Trait (defaultType A alloc.Global)}
+    `{core.clone.Clone.Trait (defaultType A alloc.Global)}
+    : Set :=
+    Entry.t K V (defaultType A alloc.Global).
+End map. End btree.
