CoqOfRust/ink/subxt.v
@@ -7,10 +7,7 @@ Require Import CoqOfRust.CoqOfRust.
 - [?] config.Config
 - [x] config.polkadot.PolkadotExtrinsicParams
 - [?] config.WithExtrinsicParams
-- [x] tx.signer.pair_signer.PairSigner
-- [x] client.online_client.OnlineClient
 - [x] utils.multi_address.MultiAddress
-- [x] utils.static_type.Static
 *)
 
 (* 
@@ -104,16 +101,12 @@ Module config.
   End extrinsic_params.
 
   (* pub struct WithExtrinsicParams<T: Config, E: ExtrinsicParams<T::Hash>> { /* private fields */ } *)
-  Unset Primitive Projections.
-  Module WithExtrinsicParams.
-    Record t (T E : Set) 
+  Parameter WithExtrinsicParams :
+    forall
+      (T E : Set)
       `{Config.Trait T}
-      (* TODO: Is this the correct way to translate the type param..? *)
-      `{extrinsic_params.ExtrinsicParams.Trait T T::type["Hash"]}
-    : Set := { }.
-  End WithExtrinsicParams.
-  Global Set Primitive Projections.
-  Definition WithExtrinsicParams := WithExtrinsicParams.t.
+      `{extrinsic_params.ExtrinsicParams.Trait T T::type["Hash"]},
+    Set.
 
   Module polkadot.
     (* pub struct PlainTip { /* private fields */ } *)
@@ -134,7 +127,14 @@ Module config.
     Definition PolkadotExtrinsicParams (T : Set) `{Config.Trait T} : Set
       := extrinsic_params.BaseExtrinsicParams T PlainTip.
   End polkadot.
-  
+
+  Module substrate.
+    Parameter BlakeTwo256 : Set.
+
+    Parameter SubstrateHeader : Set -> Set -> Set.
+
+    Parameter SubstrateExtrinsicParams : Set -> Set.
+  End substrate.
 End config.
 
 Module tx.
@@ -155,7 +155,18 @@ Module tx.
       sign : ref Self -> ref (Slice u8) -> T::type["Signature"];
     }.
   End Signer.
-  
+
+  Module signer.
+    Module pair_signer.
+      (*
+      pub struct PairSigner<T: Config, Pair> {
+          account_id: T::AccountId,
+          signer: Pair,
+      }
+      *)
+      Parameter PairSigner : Set -> Set -> Set.
+    End pair_signer.
+  End signer.
 End tx.
 
 
@@ -244,13 +255,10 @@ Module error.
 End error.
 
 Module client.
-  (* pub struct OnlineClient<T: Config> { /* private fields */ } *)
-  Unset Primitive Projections.
-  Module OnlineClient.
-    Record t : Set := { }.
-  End OnlineClient.
-  Global Set Primitive Projections.
-  Definition OnlineClient := OnlineClient.t.
+  Module online_client.
+    (* pub struct OnlineClient<T: Config> { /* private fields */ } *)
+    Parameter OnlineClient : Set -> Set.
+  End online_client.
 End client.
 
 Module utils.
@@ -275,7 +283,9 @@ Module utils.
       .
     End MultiAddress.
     Definition MultiAddress := MultiAddress.t.
+  End multi_address.
 
+  Module static_type.
     (* pub struct Static<T>(pub T); *)
     Unset Primitive Projections.
     Module Static.
@@ -285,7 +295,11 @@ Module utils.
     End Static.
     Global Set Primitive Projections.
     Definition Static := Static.t.
-  End multi_address.
+  End static_type.
+
+  Module account_id.
+    Parameter AccountId32 : Set.
+  End account_id.
 End utils.
 
 
