coq_translation/axiomatized/examples/subtle.v
@@ -265,6 +265,7 @@ End ConstantTimeEq.
 Module Impl_subtle_ConstantTimeEq_for_Slice_T.
   Section Impl_subtle_ConstantTimeEq_for_Slice_T.
     Context {T : Set}.
+    Context `{subtle.ConstantTimeEq.Trait T}.
     Definition Self := Slice T.
     
     Parameter ct_eq :
@@ -837,6 +838,9 @@ End ConditionallyNegatable.
 Module Impl_subtle_ConditionallyNegatable_for_T.
   Section Impl_subtle_ConditionallyNegatable_for_T.
     Context {T : Set}.
+    Context
+      `{subtle.ConditionallySelectable.Trait T}
+      `{core.ops.arith.Neg.Trait (ref T)}.
     Definition Self := T.
     
     Parameter conditional_negate :
@@ -886,6 +890,7 @@ Definition CtOption (T : Set) : Set := CtOption.t (T := T).
 Module Impl_core_clone_Clone_for_subtle_CtOption_T.
   Section Impl_core_clone_Clone_for_subtle_CtOption_T.
     Context {T : Set}.
+    Context `{core.clone.Clone.Trait T}.
     Definition Self := subtle.CtOption T.
     
     Parameter clone :
@@ -906,6 +911,7 @@ End Impl_core_clone_Clone_for_subtle_CtOption_T.
 Module Impl_core_marker_Copy_for_subtle_CtOption_T.
   Section Impl_core_marker_Copy_for_subtle_CtOption_T.
     Context {T : Set}.
+    Context `{core.marker.Copy.Trait T}.
     Definition Self := subtle.CtOption T.
     
     Global Instance I : core.marker.Copy.Trait Self := {
@@ -917,6 +923,7 @@ End Impl_core_marker_Copy_for_subtle_CtOption_T.
 Module Impl_core_fmt_Debug_for_subtle_CtOption_T.
   Section Impl_core_fmt_Debug_for_subtle_CtOption_T.
     Context {T : Set}.
+    Context `{core.fmt.Debug.Trait T}.
     Definition Self := subtle.CtOption T.
     
     Parameter fmt :
@@ -961,6 +968,7 @@ End Impl_core_convert_From_for_core_option_Option_T.
 Module Impl_subtle_ConditionallySelectable_for_subtle_CtOption_T.
   Section Impl_subtle_ConditionallySelectable_for_subtle_CtOption_T.
     Context {T : Set}.
+    Context `{subtle.ConditionallySelectable.Trait T}.
     Definition Self := subtle.CtOption T.
     
     Parameter conditional_select :
@@ -984,6 +992,7 @@ End Impl_subtle_ConditionallySelectable_for_subtle_CtOption_T.
 Module Impl_subtle_ConstantTimeEq_for_subtle_CtOption_T.
   Section Impl_subtle_ConstantTimeEq_for_subtle_CtOption_T.
     Context {T : Set}.
+    Context `{subtle.ConstantTimeEq.Trait T}.
     Definition Self := subtle.CtOption T.
     
     Parameter ct_eq :
